Phi_Semantics/PhiSem_CF_Return.thy
@@ -5,7 +5,7 @@ begin
 section \<open>Semantic\<close>
 
 virtual_datatype \<phi>CF_return_abnormal = \<phi>empty_abnormal +
-  ER_ret    :: \<open>VAL list\<close> \<comment> \<open>in unit of bits\<close>
+  CF_break    :: \<open>VAL list\<close> \<comment> \<open>in unit of bits\<close>
 
 print_locale \<phi>CF_return_abnormal
 
