Phi_Semantics/PhiSem_Procedure_Table.thy
@@ -1,0 +1,24 @@
+theory PhiSem_Procedure_Table
+  imports Phi_System.PhiSem_Formalization_Tools
+begin
+
+type_synonym proc_index = nat
+
+consts proc_runtime_table :: \<open>proc_index \<rightharpoonup> 'a proc\<close>
+
+specification (proc_runtime_table)
+  proc_runtime_table_inj:
+        \<open>inj_on (proc_runtime_table::proc_index \<rightharpoonup> 'a proc)
+                    (dom (proc_runtime_table::proc_index \<rightharpoonup> 'a proc))\<close>
+  proc_runtime_table_0: \<open>proc_runtime_table 0 = None\<close>
+  by (rule exI[where x=\<open>\<lambda>_. None\<close>]; simp)
+
+text \<open>A table assigning id to all procedures encountered during an execution trace.\<close>
+
+
+(*
+definition proc_of :: \<open>'a proc \<Rightarrow> proc_index proc\<close>
+  where \<open>proc_of F = (if )\<close> *)
+
+
+end
